\begin{question}
	If $f\circ g$ is surjective, then $f$ is surjective ($P$).

	\begin{proof}

		$$ P_{f\circ g}=	\forall x \in X \exists z \in Z : \, (f\circ g)(x) = z $$
		$$ P = \forall y \in Y \exists z \in Z :\, f(y) = x$$
		\begin{align*}
			P_{f\circ g}\wedge		\neg P   \implies
			     & \exists z \in Z  \forall y \in Y :\, f(y) \neq z \\
			     & \llet x \in X :\, \not\exists z : f(g(x)) = z    \\
			     & \not\exists z \in Z :\, (f\circ g)(x) = z        \\
			\sim & \neg P_{f\circ g}
		\end{align*}
		$$ \neg P \wedge P_{f\circ g} \implies \neg P_{f\circ g} \therefore P $$

	\end{proof}
\end{question}
